parametricity

coq/mergesort.v
@@ -1,8 +1,70 @@
 From mathcomp Require Import all_ssreflect.
+Declare ML Module "paramcoq".
 
 Set Implicit Arguments.
 Unset Strict Implicit.
 Unset Printing Implicit Defensive.
+
+Ltac destruct_reflexivity := 
+  intros ; repeat match goal with 
+    | [ x : _ |- _ = _ ] => destruct x; reflexivity; fail
+  end.
+
+Ltac destruct_construct x := 
+    (destruct x; [ constructor 1 ]; auto; fail)
+ || (destruct x; [ constructor 1 | constructor 2 ]; auto; fail)
+ || (destruct x; [ constructor 1 | constructor 2 | constructor 3]; auto; fail).
+
+Ltac unfold_cofix := intros; match goal with 
+ [ |- _ = ?folded ] =>  
+    let x := fresh "x" in 
+    let typ := type of folded in 
+    (match folded with _ _ => pattern folded | _ => pattern folded at 2 end);
+    match goal with [ |- ?P ?x ] => 
+    refine (let rebuild : typ -> typ := _ in 
+            let path : rebuild folded = folded := _ in  
+            eq_rect _ P _ folded path) end; 
+    [ intro x ; destruct_construct x; fail 
+    | destruct folded; reflexivity
+    | reflexivity]; fail
+end.
+
+Ltac destruct_with_nat_arg_pattern x :=
+  pattern x;
+  match type of x with 
+   | ?I 0 => refine (let gen : forall m (q : I m), 
+     (match m return I m -> Type with 
+         0 => fun p => _ p
+     | S n => fun _  => unit end q) := _ in gen 0 x)     
+   | ?I (S ?n) => refine (let gen : forall m (q : I m), 
+     (match m return I m -> Type with 
+         0 => fun _  => unit 
+     | S n => fun p => _ p end q) := _ in gen (S n) x)
+  end; intros m q; destruct q.
+
+Ltac destruct_reflexivity_with_nat_arg_pattern := 
+  intros ; repeat match goal with 
+    | [ x : _ |- _ = _ ] => destruct_with_nat_arg_pattern x; reflexivity; fail
+  end.
+ 
+Global Parametricity Tactic := ((destruct_reflexivity; fail)
+                            || (unfold_cofix; fail) 
+                            || (destruct_reflexivity_with_nat_arg_pattern; fail)
+                            ||  auto).
+
+Parametricity bool.
+Parametricity list.
+
+Lemma bool_R_refl b1 b2 : b1 = b2 -> bool_R b1 b2.
+Proof. by case: b1 => <-; constructor. Qed.
+
+Lemma map_rel_map A B (f : A -> B) (l : seq A) :
+  list_R (fun x y => f x = y) l (map f l).
+Proof. by elim: l; constructor. Qed.
+
+Lemma rel_map_map A B (f : A -> B) (l : seq A) (fl : seq B) :
+  list_R (fun x y => f x = y) l fl -> fl = map f l.
+Proof. by elim/list_R_ind: l fl / => //= ? ? <- ? ? _ ->. Qed.
 
 Definition condrev (T : Type) (r : bool) (xs : seq T) : seq T :=
   if r then rev xs else xs.
@@ -23,24 +85,36 @@ Fixpoint merge_sort_pop s1 stack :=
   if stack is s2 :: stack' then merge_sort_pop (merge leT s2 s1) stack' else s1.
 
 Fixpoint merge_sort_rec (stack : seq (seq T)) x s :=
-  if s is y :: s then
-    merge_sort_rec' stack (leT x y) [:: x] y s
-  else
-    merge_sort_pop [:: x] stack
-with
-merge_sort_rec' (stack : seq (seq T)) (mode : bool) acc x s :=
-  if s is y :: s then
-    if leT x y == mode then
-      merge_sort_rec' stack mode (x :: acc) y s
+  let inner_rec := fix inner_rec mode acc x s :=
+    if s is y :: s then
+      if eqb (leT x y) mode then
+        inner_rec mode (x :: acc) y s
+      else
+        let stack := merge_sort_push (condrev mode (x :: acc)) stack in
+        merge_sort_rec stack y s
     else
-      let stack' := merge_sort_push (condrev mode (x :: acc)) stack in
-      merge_sort_rec stack' y s
-  else
-    merge_sort_pop (condrev mode (x :: acc)) stack.
+      merge_sort_pop (condrev mode (x :: acc)) stack
+  in
+  if s is y :: s then
+    inner_rec (leT x y) [:: x] y s else merge_sort_pop [:: x] stack.
 
 Definition sort s := if s is x :: s then merge_sort_rec [::] x s else [::].
 
 End SortSeq.
+
+Parametricity Recursive sort.
+
+Lemma map_sort (T T' : Type) (f : T' -> T) (leT' : rel T') (leT : rel T) :
+  {mono f : x y / leT' x y >-> leT x y} ->
+  {morph map f : s1 / sort leT' s1 >-> sort leT s1}.
+Proof.
+move=> leT_mono xs; apply/esym/rel_map_map/sort_R/map_rel_map.
+by move=> ? ? <- ? ? <-; apply/bool_R_refl/esym/leT_mono.
+Qed.
+
+Lemma sort_map (T T' : Type) (f : T' -> T) (leT : rel T) (s : seq T') :
+  sort leT (map f s) = map f (sort (relpre f leT) s).
+Proof. exact/esym/map_sort. Qed.
 
 End CBN.
 
@@ -91,25 +165,38 @@ Fixpoint merge_sort_pop
       merge_sort_pop zs stack (~~ mode)
   end.
 
-Fixpoint merge_sort_rec (stack : seq (seq T)) x s :=
-  if s is y :: s then
-    merge_sort_rec' stack (leT x y) [:: x] y s
-  else
-    merge_sort_pop [:: x] stack false
-with
-merge_sort_rec' (stack : seq (seq T)) (mode : bool) acc x s :=
-  if s is y :: s then
-    if leT x y == mode then
-      merge_sort_rec' stack mode (x :: acc) y s
+Fixpoint merge_sort_rec (stack : seq (seq T)) (x : T) (s : seq T) : seq T :=
+  let inner_rec := fix inner_rec mode acc x s :=
+    if s is y :: s then
+      if eqb (leT x y) mode then
+        inner_rec mode (x :: acc) y s
+      else
+        let stack := merge_sort_push (condrev mode (x :: acc)) stack false in
+        merge_sort_rec stack y s
     else
-      let stack' := merge_sort_push (condrev mode (x :: acc)) stack false in
-      merge_sort_rec stack' y s
-  else
-    merge_sort_pop (condrev mode (x :: acc)) stack false.
-      
-Definition sort s := if s is x :: s then merge_sort_rec [::] x s else [::].
+      merge_sort_pop (condrev mode (x :: acc)) stack false
+  in
+  if s is y :: s then
+    inner_rec (leT x y) [:: x] y s else merge_sort_pop [:: x] stack false.
+
+Definition sort s : seq T :=
+  if s is x :: s then merge_sort_rec [::] x s else [::].
 
 End SortSeq.
+
+Parametricity Recursive sort.
+
+Lemma map_sort (T T' : Type) (f : T' -> T) (leT' : rel T') (leT : rel T) :
+  {mono f : x y / leT' x y >-> leT x y} ->
+  {morph map f : s1 / sort leT' s1 >-> sort leT s1}.
+Proof.
+move=> leT_mono xs; apply/esym/rel_map_map/sort_R/map_rel_map.
+by move => ? ? <- ? ? <-; apply/bool_R_refl/esym/leT_mono.
+Qed.
+
+Lemma sort_map (T T' : Type) (f : T' -> T) (leT : rel T) (s : seq T') :
+  sort leT (map f s) = map f (sort (relpre f leT) s).
+Proof. exact/esym/map_sort. Qed.
 
 End CBV.
 
